Various cleanups

LeanBoogie/Denotation.lean
@@ -25,8 +25,7 @@ def cgoto : Bool -> Fin b -> Fin b -> ITree E (Fin b ⊕ Unit)
 | c, t, e => if c then (.ret (.inl t)) else (.ret (.inl e))
 
 class ToITree (α : Type) (E : Type -> Type) (R : Type) where
-  -- TODO: do we need E'?
-  toITree : α -> ITree (E & E') R
+  toITree : α -> ITree E R
 
 -- TODO: don't need separate constructors?
 def denoteLiteral : Literal A -> TyA A
@@ -34,6 +33,10 @@ def denoteLiteral : Literal A -> TyA A
 | .boolL b => b
 | .bvL bv => bv
 | .realL r => r
+
+def denoteUnaryOp : UnaryOp A -> TyA A -> TyA A
+| .notB, b => ¬b
+| .negI, n => -n
 
 --noncomputable
 def denoteBinaryOp : BinaryOp A -> TyA A -> TyA A -> TyA A
@@ -52,38 +55,50 @@ def denoteBinaryOp : BinaryOp A -> TyA A -> TyA A -> TyA A
 | .equiv, a, b => a = b
 
 def denoteRelationOp : (BEq (TyA A)) -> RelationOp A -> TyA A -> TyA A -> Bool
-| _, .eq, a, b => a == b
-| _, .neq, a, b => a != b
+| _, .eq, a, b    => a == b
+| _, .neq, a, b   => a != b
 | _, .lessI, x, y => x < y
 
-def denoteAppliable [Monad m] : Appliable A B -> m (TyA A -> TyA B)
-| .binop op => pure (denoteBinaryOp op)
-| .unop op => pure (denoteUnaryOp op)
-| .relop eq op => pure (denoteRelationOp eq op)
-| .mapSelect => pure (λ x => x)
+def denoteAppliable : Appliable A B -> TyA A -> TyA B
+| .binop op    => denoteBinaryOp op
+| .unop op     => denoteUnaryOp op
+| .relop eq op => denoteRelationOp eq op
+| .mapSelect   => id
 
--- We can denote an expression using an arbitrary function to retrieve
--- the value of a variable. We make it monadic so that it can, if desired
--- work in a state or ITree monad.
-def denoteExpr [Monad m] : Ctx m Γ -> Expr Γ A -> m (TyA A)
-| _, .lit l => pure (denoteLiteral l)
-| γ, .apply a e => do
-  pure ((<- denoteAppliable a) (<- denoteExpr γ e))
-| γ, .applyExpr fe e => do
-  pure ((<- denoteExpr γ fe) (<- denoteExpr γ e))
-| γ, .var x => γ x
+def denoteExpr : ConA Γ -> Expr Γ A -> TyA A
+| _, .lit l          => denoteLiteral l
+| γ, .apply a e      => (denoteAppliable a) (denoteExpr γ e)
+| γ, .applyExpr fe e => (denoteExpr γ fe) (denoteExpr γ e)
+| γ, .var x          => ConA.get γ x
+| γ, .lambda e       => λ x => denoteExpr (x, γ) e
 
 -- Within an ITree, we don't need to pass around a context, and can just
--- use Mem.read.
-def denoteExprI : Expr Γ A -> ITree (Mem Γ) (TyA A) :=
-  denoteExpr Mem.read
+-- use Mem.readAll.
+def denoteExprI {A : Ty} {Γ : Con} (e: Expr Γ A) : ITree (Mem Γ) (TyA A) := do
+  let γ <- Mem.readAll
+  return (denoteExpr γ e)
+
+def denoteFormula : ConA Γ -> Formula Γ -> Prop
+| γ, .forallF p => forall x, denoteFormula (x, γ) p
+| γ, .existsF p => exists x, denoteFormula (x, γ) p
+| γ, .andF p q  => denoteFormula γ p /\ denoteFormula γ q
+| γ, .orF p q  => denoteFormula γ p \/ denoteFormula γ q
+| γ, .impF p q  => denoteFormula γ p -> denoteFormula γ q
+| γ, .eqF p q   => denoteFormula γ p = denoteFormula γ q
+| γ, .eqE e1 e2   => denoteExpr γ e1 = denoteExpr γ e2
+| _, .litF b    => b
+| γ, .boolF e   => denoteExpr γ e
+
+def denotePropExprI (p: Formula Γ) : ITree (Mem Γ) Prop := do
+  let γ <- Mem.readAll
+  .pure (denoteFormula γ p)
 
 instance exprITree : ToITree (Expr Γ A) (Mem Γ) (TyA A) where
-  toITree e := denoteExprI e
+  toITree := denoteExprI
 
 def denotePassiveCommand : PassiveCommand Γ -> ITree (Mem Γ & AmAt) Unit
-| .assert e => do assert (<- denoteExprI e)
-| .assume e => do assume (<- denoteExprI e)
+| .assert e => do assert (<- denotePropExprI e)
+| .assume e => do assume (<- denotePropExprI e)
 
 def denoteCommand : Command Γ -> ITree (Mem Γ & AmAt & E) Unit
 | .passive p => denotePassiveCommand p
@@ -130,3 +145,24 @@ def denoteStructuredCommands :
   | .inl b => .pure (.inl b)
   | .inr _ => denoteStructuredCommands cs
 end
+
+def denoteUnstructuredProcedure
+   (p: Procedure (Command Γ) Unit Γ)
+   (args: ConA p.inParams) :
+   -- TODO: make more effect polymorphic
+   -- TODO: add inputs to state
+   -- TODO: add locals to state
+   -- TODO: add outputs to state
+   -- TODO: read outputs from state
+   ITree (Mem Γ & AmAt & Choice) (ConA p.outParams) := do
+    -- Initialize local and output variables with default values
+    let globalState : ConA Γ <- liftM Mem.readAll
+    let locState : ConA p.locals := default
+    let outState : ConA p.outParams := default
+    let addlState := args ++ locState ++ outState
+    -- Run blocks
+    -- TODO: run in totalState instead of Γ
+    denoteBlocks p.body (cast sorry 0)
+    -- Read output variables
+    let outState' : ConA p.outParams := sorry
+    return outState'
