LeanBoogie/Syntax.lean
@@ -14,10 +14,6 @@ inductive UnaryOp : Ty -> Type
 | notB : UnaryOp .bool
 | negI : UnaryOp .int
 
-def denoteUnaryOp : UnaryOp A -> TyA A -> TyA A
-| .notB, b => ¬b
-| .negI, n => -n
-
 inductive BinaryOp : Ty -> Type
 | addI : BinaryOp .int
 | subI : BinaryOp .int
@@ -49,15 +45,31 @@ inductive Expr : Con -> Ty -> Type
 | var : Var Γ A -> Expr Γ A
 | apply : Appliable A B -> Expr Γ A -> Expr Γ B
 | applyExpr : Expr Γ (.map A B) -> Expr Γ A -> Expr Γ B
+| lambda : Expr (A :: Γ) B -> Expr Γ (.map A B)
+
+inductive Formula : Con -> Type
+| forallF : Formula (ty :: Γ) -> Formula Γ
+| existsF : Formula (ty :: Γ) -> Formula Γ
+| boolF : Expr Γ .bool -> Formula Γ
+-- Grr. I don't like needing separate boolean and formula operators, but
+-- this works out most cleanly.
+| andF : Formula Γ -> Formula Γ -> Formula Γ
+| orF : Formula Γ -> Formula Γ -> Formula Γ
+| impF : Formula Γ -> Formula Γ -> Formula Γ
+| eqF : Formula Γ -> Formula Γ -> Formula Γ
+| eqE : Expr Γ A -> Expr Γ A -> Formula Γ
+| litF : Bool -> Formula Γ
 
 abbrev mkUn (op : UnaryOp A) (l : Expr Γ A) : Expr Γ A :=
   .apply (.unop op) l
 abbrev mkBin (op : BinaryOp A) (l : Expr Γ A) (r : Expr Γ A) : Expr Γ A :=
   .applyExpr (.apply (.binop op) l) r
+abbrev mkRel (beq: BEq (TyA A)) (op : RelationOp A) (l : Expr Γ A) (r : Expr Γ A) : Expr Γ .bool :=
+  .applyExpr (.apply (.relop beq op) l) r
 
 inductive PassiveCommand : Con -> Type
-| assert : Expr Γ .bool -> PassiveCommand Γ
-| assume : Expr Γ .bool -> PassiveCommand Γ
+| assert : Formula Γ -> PassiveCommand Γ
+| assume : Formula Γ -> PassiveCommand Γ
 
 inductive Command : Con -> Type
 | assign : (v : Var Γ A) -> Expr Γ A -> Command Γ
@@ -78,7 +90,8 @@ structure Block (C: Type) (S: Type) (b : Nat) (Γ : Con) where
   structuredCmd : S
   transferCmd : TransferCommand b Γ
 
-abbrev SimpleBlock Γ b := Block (PassiveCommand Γ) Unit b Γ
+abbrev PassiveBlock Γ b := Block (PassiveCommand Γ) Unit b Γ
+abbrev SimpleBlock Γ b := Block (Command Γ) Unit b Γ
 
 inductive StructuredCommand (b: Nat) : Con -> Type
 | ite : Expr Γ .bool ->
@@ -94,10 +107,10 @@ inductive StructuredCommand (b: Nat) : Con -> Type
 
 abbrev BigBlock (b : Nat) (Γ : Con) := Block (Command Γ) (StructuredCommand b Γ) b Γ
 
-abbrev Command.assert (p : Expr Γ .bool) : Command Γ := .passive (.assert p)
-abbrev Command.assume (p : Expr Γ .bool) : Command Γ := .passive (.assume p)
+abbrev Command.assert (p : Formula Γ) : Command Γ := .passive (.assert p)
+abbrev Command.assume (p : Formula Γ) : Command Γ := .passive (.assume p)
 -- abbrev Command.goto (ns : List (Fin b)) : Command b Γ := .passive (.goto ns)
-abbrev Command.skip : Command Γ := .assume (.lit (.boolL True))
+abbrev Command.skip : Command Γ := .assume (.boolF (.lit (.boolL True)))
 
 structure Axiom (Γ : Con) where
   name : Option Lean.Name
@@ -120,14 +133,16 @@ structure Variable where
   ty : Ty
 
 structure Procedure (C: Type) (S: Type) (Γ : Con) where
+  -- Γ describes globals
   name : Lean.Name
   b : Nat
+  binhabited : b > 0
   effects : Type -> Type
   inParams : Con
   locals : Con
   outParams : Con
   -- TODO: contracts
-  body : Fin b -> Block C S b (Γ ++ inParams ++ locals ++ outParams)
+  body : Fin b -> Block C S b (Γ /- ++ inParams ++ locals ++ outParams-/)
 
 inductive Declaration (Γ : Con) : Type 1
 | axiomDecl : Axiom Γ -> Declaration Γ
@@ -139,8 +154,3 @@ inductive Declaration (Γ : Con) : Type 1
 structure Program where
   Γ : Con
   declarations : Declaration Γ
-
-abbrev Ctx m [Monad m] (Γ : Con) := {A : Ty} -> Var Γ A -> m (TyA A)
-abbrev Ctx.get [Monad m] : Ctx m Γ -> Var Γ A -> m (TyA A)
-| γ => γ
-abbrev Ctx.extend [Monad m] : Ctx m Γ -> TyA A -> Ctx m (A :: Γ) := sorry
