LeanBoogie/WP.lean
@@ -12,38 +12,36 @@ open LeanBoogie
 
 namespace LeanBoogie
 
-def wpPassiveS : PassiveCommand Γ -> Expr Γ .bool -> Expr Γ .bool
-| .assert P, Q => mkBin .and P Q
-| .assume P, Q => mkBin .imp P Q
+def wpPassiveS : PassiveCommand Γ -> Formula Γ -> Formula Γ
+| .assert P, Q => .andF P Q
+| .assume P, Q => .impF P Q
 
-def wpPassiveCommandsS : List (PassiveCommand Γ) -> Expr Γ .bool -> Expr Γ .bool
+def wpPassiveCommandsS : List (PassiveCommand Γ) -> Formula Γ -> Formula Γ
 | [], Q => Q
 | c :: cs, Q => wpPassiveS c (wpPassiveCommandsS cs Q)
 
-def wpTransferCommandS : (Fin b -> Expr Γ .bool) -> TransferCommand b Γ -> Expr Γ .bool -> Expr Γ .bool
-| blkVar, .goto ls, _ => List.foldl (λ a b => mkBin .and a b) (.lit (.boolL True)) (List.map blkVar ls)
+def wpTransferCommandS : (Fin b -> Formula Γ) -> TransferCommand b Γ -> Formula Γ -> Formula Γ
+| blkVar, .goto ls, _ => List.foldl (λ a b => .andF a b) (.litF true) (List.map blkVar ls)
 | _, .ret, Q => Q
 
-def wpPassiveBlockS (blkVar: Fin b -> Expr Γ .bool) (blk: SimpleBlock Γ b) (Q: Expr Γ .bool) : Expr Γ .bool :=
-  mkBin .equiv (blkVar blk.label) (wpPassiveCommandsS blk.simpleCmds (wpTransferCommandS blkVar blk.transferCmd Q))
+def wpPassiveBlockS (blkVar: Fin b -> Formula Γ) (blk: PassiveBlock Γ b) (Q: Formula Γ) : Formula Γ :=
+  .eqF (blkVar blk.label) (wpPassiveCommandsS blk.simpleCmds (wpTransferCommandS blkVar blk.transferCmd Q))
 
-def wpPassiveD : Ctx Id Γ -> PassiveCommand Γ -> Prop -> Prop
-| γ, .assert P, Q => (Id.run (denoteExpr γ P)) ∧ Q
-| γ, .assume P, Q => (Id.run (denoteExpr γ P)) → Q
+def wpPassiveD : ConA Γ -> PassiveCommand Γ -> Prop -> Prop
+| γ, .assert P, Q => denoteFormula γ P ∧ Q
+| γ, .assume P, Q => denoteFormula γ P → Q
 
 theorem wpPassiveDCorrect :
   { Γ : Con } ->
-  { γ : Ctx Id Γ } ->
-  { Q : Expr Γ .bool } ->
+  { γ : ConA Γ } ->
+  { Q : Formula Γ } ->
   ( c : PassiveCommand Γ ) ->
-  wpPassiveD γ c (Id.run (denoteExpr γ Q)) = Id.run (denoteExpr γ (wpPassiveS c Q)) :=
+  wpPassiveD γ c (denoteFormula γ Q) = (denoteFormula γ (wpPassiveS c Q)) :=
   by intros Γ γ Q c
      unfold wpPassiveS wpPassiveD
-     unfold mkBin
-     cases c <;>
-       (simp [denoteExpr, denoteAppliable, denoteBinaryOp] ; repeat rw [Id.run])
+     cases c <;> simp [denoteExpr, denoteFormula]
 
-def wpPassiveCommandsD : Ctx Id Γ -> List (PassiveCommand Γ) -> Prop -> Prop
+def wpPassiveCommandsD : ConA Γ -> List (PassiveCommand Γ) -> Prop -> Prop
 | _, [], Q => Q
 | γ, c :: cs, Q => wpPassiveD γ c (wpPassiveCommandsD γ cs Q)
 
@@ -51,5 +49,5 @@ def wpTransferCommandD : (Fin b -> Prop) -> TransferCommand b Γ -> Prop -> Prop
 | blkVar, .goto ls, _ => List.foldl (λ a b => a ∧ b) True (List.map blkVar ls)
 | _, .ret, Q => Q
 
-def wpPassiveBlockD (γ : Ctx Id Γ) (blkVar: Fin b -> Prop) (blk: SimpleBlock Γ b) (Q: Prop) : Prop :=
+def wpPassiveBlockD (γ : ConA Γ) (blkVar: Fin b -> Prop) (blk: PassiveBlock Γ b) (Q: Prop) : Prop :=
   blkVar blk.label = wpPassiveCommandsD γ blk.simpleCmds (wpTransferCommandD blkVar blk.transferCmd Q)
